wip: first pass at elaboration for magmas

Rz/Algebra/PCA.lean
@@ -1,8 +1,6 @@
 /-
 # Partial Combinatory Algebras
 -/
-import Mathlib.Tactic.Simps.Basic
-import Mathlib.Data.Part
 import Mathlib.Data.List.Indexes
 
 import Rz.Data.Bwd
@@ -13,79 +11,36 @@ import Rz.Syntax.Magma
 universe u v w
 variable {α β : Type u}
 
-/-- Notation typeclass for `a ⋆ b`. -/
-@[notation_class]
-class HasAp (α : Type u) (β : Type v) (γ : outParam (Type w)) where
-  /-- `a ⋆ b` computes to the application of `a` and `b`.
-  The meaning of this notation is type-dependent. -/
-  hAp : α → β → γ
-
-@[inherit_doc] infixl:60 " ⋆ " => HasAp.hAp
-
-/-- Extends application to an operation on partial elements. -/
-instance instPartLeft [H : HasAp α β (Part γ)] : HasAp (Part α) β (Part γ) where
-  hAp a b := do
-    Part.bind a (fun a => H.hAp a b)
-
-@[simp] theorem ap_some_left [HasAp α β (Part γ)] (a : α) (b : β) : Part.some a ⋆ b = a ⋆ b := by
-  simp [HasAp.hAp]
-
-@[simp] theorem ap_bind_left_dom [HasAp α β (Part γ)] (a : Part α) (b : β) : a ⋆ b ↓ ↔ ∃ h : a ↓, a.get h ⋆ b ↓ := by
-  simp [HasAp.hAp]
-
-instance instPartRight [H : HasAp α β (Part γ)] : HasAp α (Part β) (Part γ) where
-  hAp a b := do
-    Part.bind b (fun b => H.hAp a b)
-
-@[simp] theorem ap_some_right [HasAp α β (Part γ)] (a : α) (b : β) : a ⋆ Part.some b = a ⋆ b := by
-  simp [HasAp.hAp]
-
-@[simp] theorem ap_bind_right_dom [HasAp α β (Part γ)] (a : α) (b : Part β) : a ⋆ b ↓ ↔ ∃ h : b ↓, a ⋆ b.get h ↓ := by
-  simp [HasAp.hAp]
-
-/-- Extends application to (snoc) lists. -/
-instance [H : HasAp α β (Part α)] : HasAp α (Bwd β) (Part α) where
-  hAp a bs := Bwd.foldBwdM H.hAp a bs
-
-@[simp] theorem aps_bwd_nil [HasAp α β (Part α)] (a : α) : a ⋆ (Bwd.nil : Bwd β) = a := by
-  simp [HasAp.hAp]
-
-@[simp] theorem aps_bwd_cons [HasAp α β (Part α)] (a : α) (bs : Bwd β) (b : β) : a ⋆ (bs :# b) = (a ⋆ bs) ⋆ b := by
-  simp [HasAp.hAp]
-
-@[simp] theorem aps_list_append [HasAp α β (Part α)] (a : α) (as bs : Bwd β) : a ⋆ (as ++ bs) = (a ⋆ as) ⋆ bs := by
-  simp [HasAp.hAp]
-
-
 /-- Partial Applicative Structures. -/
 class PAS (α : Type u) where
-  ap : α → α → Part α
+  Eval : FreeMagma α 0 → α → Prop
+  functional : (e : FreeMagma α 0) → (a a' : α) → Eval e a → Eval e a' → a = a'
 
-@[default_instance]
-instance instPasApply [PAS α] : HasAp α α (Part α) where
-  hAp := PAS.ap
+infix:60 " ⇓ " => PAS.Eval
 
-/-- Reduce a word in the free magma using `PAS.ap`. -/
-def PAS.eval [PAS α] (ρ : Bwd α) : FreeMagma α ρ.length → Part α :=
-  FreeMagma.foldM (fun x => pure (Bwd.get ρ x)) pure PAS.ap
+def PAS.Defined [PAS α] (e : FreeMagma α 0) : Prop := ∃ (a : α), PAS.Eval e a
 
-@[simp] theorem PAS.var [PAS α] (ρ : Bwd α) (x : Fin ρ.length) : PAS.eval ρ (.var x) = ρ.get x := rfl
-@[simp] theorem PAS.eval_const [PAS α] (ρ : Bwd α) (a : α) : PAS.eval ρ (.const a) = a := rfl
-@[simp] theorem PAS.op [PAS α] (ρ : Bwd α) (e₁ e₂ : FreeMagma α ρ.length) : PAS.eval ρ (.op e₁ e₂) = PAS.eval ρ e₁ ⋆ PAS.eval ρ e₂ := rfl
+notation:60 e " ↓" => PAS.Defined e
 
+-- @[default_instance]
+-- instance instPasApply [PAS α] : HasAp α α (Part α) where
+--   hAp := PAS.ap
 
--- @[simp] theorem PAS.eval_const_dom [PAS α] (a : α) (ρ : List α) : PAS.eval ρ (.const a) ↓ := by
---   simp [PAS.eval, FreeMagma.foldM]
+-- /-- Reduce a word in the free magma using `PAS.ap`. -/
+-- def PAS.eval [PAS α] (ρ : Bwd α) : FreeMagma α ρ.length → Part α :=
+--   FreeMagma.foldM (fun x => pure (Bwd.get ρ x)) pure PAS.ap
 
--- @[simp] theorem PAS.eval_op_dom [PAS α] (ρ : List α) (e₁ e₂ : FreeMagma α ρ.length) : PAS.eval ρ (.op e₁ e₂) ↓ ↔ PAS.eval ρ e₁ ⋆ PAS.eval ρ e₂ ↓ := Iff.rfl
+-- @[simp] theorem PAS.var [PAS α] (ρ : Bwd α) (x : Fin ρ.length) : PAS.eval ρ (.var x) = ρ.get x := rfl
+-- @[simp] theorem PAS.eval_const [PAS α] (ρ : Bwd α) (a : α) : PAS.eval ρ (.const a) = a := rfl
+-- @[simp] theorem PAS.op [PAS α] (ρ : Bwd α) (e₁ e₂ : FreeMagma α ρ.length) : PAS.eval ρ (.op e₁ e₂) = PAS.eval ρ e₁ ⋆ PAS.eval ρ e₂ := rfl
 
-class PCA (α : Type u) extends PAS α where
-  rep : {n : Nat} → FreeMagma α (n + 1) → α
-  rep_dom
-    : (ρ : Bwd α) → (e : FreeMagma α (ρ.length + 1)) → rep e ⋆ ρ ↓
-  rep_eval
-    : (ρ : Bwd α) → (a : α) → (e : FreeMagma α (ρ.length + 1))
-    → rep e ⋆ ρ = PAS.eval (ρ :# a) e
+-- class PCA (α : Type u) extends PAS α where
+--   rep : {n : Nat} → FreeMagma α (n + 1) → α
+--   repDom
+--     : (ρ : Bwd α) → (e : FreeMagma α (ρ.length + 1)) → rep e ⋆ ρ ↓
+--   repEval
+--     : (ρ : Bwd α) → (a : α) → (e : FreeMagma α (ρ.length + 1))
+--     → rep e ⋆ ρ = PAS.eval (ρ :# a) e
 
 /-!
 # Completeness of the SKI basis.
@@ -97,124 +52,128 @@ class SKI (α : Type u) extends PAS α where
   /-- `k` combinator; analog of the λ-term `fun x y => x`. -/
   k : α
   /-- Applying `s` to two arguments is always defined. -/
-  sDom : (a b : α) → s ⋆ a ⋆ b ↓
-  /-- Applying `k` to one argument is always defined. -/
-  kDom : (a : α) → k ⋆ a ↓
-  /-- Characterize computational behaviour of `s`. -/
-  sEval : (a b c : α) → s ⋆ a ⋆ b ⋆ c = (a ⋆ b) ⋆ (a ⋆ c)
-  /-- Characterize computational behaviour of `k`. -/
-  kEval : (a b : α) → k ⋆ a ⋆ b = a
+  sDom : (a b : α) → [magma|| s a b |] ↓
+  kDom : (a : α) → [magma|| k a |] ↓
 
-  /-- `i` combinator; can be derived from `s` and `k` -/
-  i : α := (s ⋆ k ⋆ k).get (sDom k k)
-  /-- Characterize computational behaviour of `i`. -/
-  iEval : (a : α) → i ⋆ a = a
+  sEval : (a b c : α) (v : α) → [magma|| s a b c |]
 
+  -- sDom : (a b : α) → s ⋆ a ⋆ b ↓
+  -- /-- Applying `k` to one argument is always defined. -/
+  -- kDom : (a : α) → k ⋆ a ↓
+  -- /-- Characterize computational behaviour of `s`. -/
+  -- sEval : (a b c : α) → s ⋆ a ⋆ b ⋆ c = (a ⋆ b) ⋆ (a ⋆ c)
+  -- /-- Characterize computational behaviour of `k`. -/
+  -- kEval : (a b : α) → k ⋆ a ⋆ b = a
 
-namespace SKI
+  -- /-- `i` combinator; can be derived from `s` and `k` -/
+  -- i : α := (s ⋆ k ⋆ k).get (sDom k k)
+  -- /-- Characterize computational behaviour of `i`. -/
+  -- iEval : (a : α) → i ⋆ a = a
 
-@[simp] def s_dom_1 [SKI α] (a : α) : s ⋆ a ↓ := (SKI.sDom a k).fst
-@[simp] def s_dom_2 [SKI α] (a b : α) : s ⋆ a ⋆ b ↓ := SKI.sDom a b
-@[simp] def s_dom_2_get [SKI α] (a b : α) : (s ⋆ a).get (s_dom_1 a) ⋆ b ↓ := (SKI.sDom a b).snd
-@[simp] def k_dom_1 [SKI α] (a : α) : k ⋆ a ↓ := SKI.kDom a
+-- namespace SKI
 
-/-- Bracket abstraction. -/
-def abs [SKI α] : FreeMagma α (n + 1) → FreeMagma α n
-| .var x =>
-  if h : x = 0 then
-    .const i
-  else
-    .op (.const k) (.var (Fin.pred x h))
-| .const a =>
-  .op (.const k) (.const a)
-| .op e₁ e₂ =>
-  .op (.op (.const s) (abs e₁)) (abs e₂)
+-- @[simp] def s_dom_1 [SKI α] (a : α) : s ⋆ a ↓ := (SKI.sDom a k).fst
+-- @[simp] def s_dom_2 [SKI α] (a b : α) : s ⋆ a ⋆ b ↓ := SKI.sDom a b
+-- @[simp] def s_dom_2_get [SKI α] (a b : α) : (s ⋆ a).get (s_dom_1 a) ⋆ b ↓ := (SKI.sDom a b).snd
+-- @[simp] def k_dom_1 [SKI α] (a : α) : k ⋆ a ↓ := SKI.kDom a
 
-/-- Iterated bracket abstraction. -/
-def absn [SKI α] {m : Nat} (n : Nat) (e : FreeMagma α (m + n)) : FreeMagma α m :=
-match n with
-| 0 => e
-| n+1 => absn n (abs e)
+-- /-- Bracket abstraction. -/
+-- def abs [SKI α] : FreeMagma α (n + 1) → FreeMagma α n
+-- | .var x =>
+--   if h : x = 0 then
+--     .const i
+--   else
+--     .op (.const k) (.var (Fin.pred x h))
+-- | .const a =>
+--   .op (.const k) (.const a)
+-- | .op e₁ e₂ =>
+--   .op (.op (.const s) (abs e₁)) (abs e₂)
 
-def eval_abs_dom [SKI α] (ρ : Bwd α) (e : FreeMagma α (ρ.length + 1)) : PAS.eval ρ (abs e) ↓ := by
-  induction e <;> simp [abs]
-  case var x =>
-    cases (decEq x 0)
-    case isTrue h =>
-      simp [dif_pos h]
-    case isFalse h =>
-      simp [dif_neg h]
-  case op e₁ e₂ e₁_ih e₂_ih =>
-    exists e₁_ih
-    exists e₂_ih
-    apply s_dom_2_get
+-- /-- Iterated bracket abstraction. -/
+-- def absn [SKI α] {m : Nat} (n : Nat) (e : FreeMagma α (m + n)) : FreeMagma α m :=
+-- match n with
+-- | 0 => e
+-- | n+1 => absn n (abs e)
 
-def eval_absn_dom [SKI α] (n : Nat) (ρ : Bwd α) (e : FreeMagma α (ρ.length + n + 1)) : PAS.eval ρ (absn (n + 1) e) ↓ := by
-  induction n <;> simp [absn]
-  case zero =>
-    exact (eval_abs_dom ρ e)
-  case succ n ih =>
-    apply ih
+-- def eval_abs_dom [SKI α] (ρ : Bwd α) (e : FreeMagma α (ρ.length + 1)) : PAS.eval ρ (abs e) ↓ := by
+--   induction e <;> simp [abs]
+--   case var x =>
+--     cases (decEq x 0)
+--     case isTrue h =>
+--       simp [dif_pos h]
+--     case isFalse h =>
+--       simp [dif_neg h]
+--   case op e₁ e₂ e₁_ih e₂_ih =>
+--     exists e₁_ih
+--     exists e₂_ih
+--     apply s_dom_2_get
 
-def rep [SKI α] (ρ : Bwd α) (n : Nat) (e : FreeMagma α (ρ.length + n + 1)) : α :=
-  (PAS.eval ρ (absn (n + 1) e)).get (eval_absn_dom n ρ e)
+-- def eval_absn_dom [SKI α] (n : Nat) (ρ : Bwd α) (e : FreeMagma α (ρ.length + n + 1)) : PAS.eval ρ (absn (n + 1) e) ↓ := by
+--   induction n <;> simp [absn]
+--   case zero =>
+--     exact (eval_abs_dom ρ e)
+--   case succ n ih =>
+--     apply ih
 
-def rep_dom [SKI α] (ρ σ : Bwd α) (e : FreeMagma α (ρ.length + σ.length + 1)) : rep ρ σ.length e ⋆ σ ↓ := by
-  induction σ <;> simp [rep, absn]
-  case nil =>
-    exact (eval_abs_dom ρ e)
-  case snoc σ a ih =>
-    exists (ih (abs e))
-    sorry
-    -- sorry
-    -- exact (eval_absn_dom _ ρ e)
-end SKI
+-- def rep [SKI α] (ρ : Bwd α) (n : Nat) (e : FreeMagma α (ρ.length + n + 1)) : α :=
+--   (PAS.eval ρ (absn (n + 1) e)).get (eval_absn_dom n ρ e)
 
-
-
--- def PAS.rep_dom [PAS α]
---   (s k i : α)
---   (s_def : (a b : α) → (s ⋆ a ⋆ b) ↓)
---   (k_def : (a : α) → (k ⋆ a) ↓)
---   (ρ σ : Bwd α)
---   (e : FreeMagma α (ρ.length + σ.length + 1))
---   : (PAS.rep s k i s_def k_def ρ σ.length e) ⋆ σ ↓ := by
---   unfold rep
---   induction σ
+-- def rep_dom [SKI α] (ρ σ : Bwd α) (e : FreeMagma α (ρ.length + σ.length + 1)) : rep ρ σ.length e ⋆ σ ↓ := by
+--   induction σ <;> simp [rep, absn]
 --   case nil =>
---     simp
---     exact (PAS.eval_absn_dom s k i s_def k_def ρ e)
+--     exact (eval_abs_dom ρ e)
 --   case snoc σ a ih =>
---     simp [absn]
+--     exists (ih (abs e))
 --     sorry
---     -- exists (ih (abs s k i e))
-    -- sorry
+--     -- sorry
+--     -- exact (eval_absn_dom _ ρ e)
+-- end SKI
 
--- def PCA.k [PCA α] : α :=
---   PCA.rep FreeMagma.k
 
--- def PCA.s [PCA α] : α :=
---   PCA.rep FreeMagma.s
 
--- def PCA.i [PCA α] : α :=
---   (PAS.aps PCA.s [PCA.k, PCA.k]).get (PCA.rep_def FreeMagma.s [PCA.k, PCA.k] (by simp))
+-- -- def PAS.rep_dom [PAS α]
+-- --   (s k i : α)
+-- --   (s_def : (a b : α) → (s ⋆ a ⋆ b) ↓)
+-- --   (k_def : (a : α) → (k ⋆ a) ↓)
+-- --   (ρ σ : Bwd α)
+-- --   (e : FreeMagma α (ρ.length + σ.length + 1))
+-- --   : (PAS.rep s k i s_def k_def ρ σ.length e) ⋆ σ ↓ := by
+-- --   unfold rep
+-- --   induction σ
+-- --   case nil =>
+-- --     simp
+-- --     exact (PAS.eval_absn_dom s k i s_def k_def ρ e)
+-- --   case snoc σ a ih =>
+-- --     simp [absn]
+-- --     sorry
+-- --     -- exists (ih (abs s k i e))
+--     -- sorry
 
--- def PCA.abs [PCA α] : FreeMagma α (n + 1) → FreeMagma α n
--- | .var 0 => .const PCA.i
--- | .var ⟨ x+1 , h ⟩ => .op (.const PCA.k) (.var ⟨ x , by omega ⟩)
--- | .const a => .op (.const PCA.k) (.const a)
--- | .op l r => .op (.op (.const PCA.s) (PCA.abs l)) (PCA.abs r)
+-- -- def PCA.k [PCA α] : α :=
+-- --   PCA.rep FreeMagma.k
 
--- def PCA.s_k_complete
---   [A : PAS α]
---   (s k i : α)
---   (s_def : (a b : α) → (s ⋆ [a, b]) ↓)
---   (k_def : (a : α) → (k ⋆ a) ↓)
---   (s_eval : (a b c : α) → KleeneEquiv (s ⋆ [a, b, c]) (A.evalClosed (.op (.op (.const a) (.const c)) (.op (.const b) (.const c)))))
---   (k_eval : (a b : α) → (k ⋆ [a, b]) = a)
---   (i_eval : (a : α) → (i ⋆ a) = a)
---   : PCA α := {
---   rep := PAS.rep s k i
---   rep_def := _
---   rep_eval := _
--- }
+-- -- def PCA.s [PCA α] : α :=
+-- --   PCA.rep FreeMagma.s
+
+-- -- def PCA.i [PCA α] : α :=
+-- --   (PAS.aps PCA.s [PCA.k, PCA.k]).get (PCA.rep_def FreeMagma.s [PCA.k, PCA.k] (by simp))
+
+-- -- def PCA.abs [PCA α] : FreeMagma α (n + 1) → FreeMagma α n
+-- -- | .var 0 => .const PCA.i
+-- -- | .var ⟨ x+1 , h ⟩ => .op (.const PCA.k) (.var ⟨ x , by omega ⟩)
+-- -- | .const a => .op (.const PCA.k) (.const a)
+-- -- | .op l r => .op (.op (.const PCA.s) (PCA.abs l)) (PCA.abs r)
+
+-- -- def PCA.s_k_complete
+-- --   [A : PAS α]
+-- --   (s k i : α)
+-- --   (s_def : (a b : α) → (s ⋆ [a, b]) ↓)
+-- --   (k_def : (a : α) → (k ⋆ a) ↓)
+-- --   (s_eval : (a b c : α) → KleeneEquiv (s ⋆ [a, b, c]) (A.evalClosed (.op (.op (.const a) (.const c)) (.op (.const b) (.const c)))))
+-- --   (k_eval : (a b : α) → (k ⋆ [a, b]) = a)
+-- --   (i_eval : (a : α) → (i ⋆ a) = a)
+-- --   : PCA α := {
+-- --   rep := PAS.rep s k i
+-- --   rep_def := _
+-- --   rep_eval := _
+-- -- }
