Rz/Syntax/Magma.lean
@@ -1,6 +1,11 @@
 /-
 # Free Magmas
 -/
+import Lean
+
+import Rz.Data.Bwd
+
+open Lean Elab Meta Term
 
 universe u v w
 
@@ -20,8 +25,76 @@ def foldM [Monad m] (v : Fin n → m β) (c : α → m β) (o : β → β → m 
   let b ← foldM v c o r
   o a b
 
-def k : FreeMagma α 2 := .var 0
 
-def s : FreeMagma α 3 := .op (.op (.var 0) (.var 2)) (.op (.var 1) (.var 2))
+/-!
+# Elaboration
+-/
 
-end FreeMagma
+/-- Extensible elaboration of magma expressions. -/
+class MagmaExpr (α : Type u) (β : outParam (Type v)) where
+  expr : {n : Nat} → α → FreeMagma β n
+
+@[default_instance]
+instance : MagmaExpr α α where
+  expr := .const
+
+declare_syntax_cat magma
+syntax ident : magma
+syntax:10 magma:10 magma:11+ : magma
+syntax "(" magma:min ")" : magma
+
+unsafe def mkMagmaVar (u : Level) (tp : Expr) (vars : TSyntaxArray `ident) (x : Ident) : TermElabM Expr := do
+  let size ← mkNumeral (mkConst ``Nat) vars.size
+  -- Check to see if the variable is bound by the `magma` binding form.
+  match Array.indexOf? vars x with
+  | some ix =>
+    -- If it is, construct a `var` with the correct de Bruijn index.
+    let x ← mkNumeral (mkApp (mkConst ``Fin) size) (vars.size - ix - 1)
+    pure (mkAppN (mkConst ``FreeMagma.var [u]) #[tp, size, x])
+  | none =>
+    -- Otherwise, elaborate `x` as an identifier, and pass it off to instance resolution.
+    let v ← mkFreshLevelMVar
+    let mvar ← mkFreshExprMVar none
+    let e ← elabIdent x mvar
+    let inst ← synthInstance (mkAppN (mkConst ``MagmaExpr [v, u]) #[mvar, tp])
+    pure (mkAppN (mkConst ``MagmaExpr.expr [v, u]) #[mvar, tp, inst, size, e])
+
+
+def mkMagmaOp (u : Level) (tp : Expr) (vars : TSyntaxArray `ident) (a : Expr) (args : Array Expr) : TermElabM Expr := do
+  let size ← mkNumeral (mkConst ``Nat) vars.size
+  pure (Array.foldl (fun acc arg => mkAppN (mkConst ``FreeMagma.op [u]) #[tp, size, acc, arg]) a args)
+
+unsafe def mkMagmaExpr (u : Level) (tp : Expr) (vars : TSyntaxArray `ident) : Syntax → TermElabM Expr
+| `(magma| $x:ident) =>
+  mkMagmaVar u tp vars x
+| `(magma| $a:magma $args:magma*) => do
+  let ea ← mkMagmaExpr u tp vars a
+  let eas ← Array.mapM (fun arg => mkMagmaExpr u tp vars arg) args
+  mkMagmaOp u tp vars ea eas
+| `(magma| ( $a )) => mkMagmaExpr u tp vars a
+| _ => throwUnsupportedSyntax
+
+
+syntax (name := magma_expr) "[magma|" ident* "|" magma "|]" : term
+
+#check BinderInfo
+
+@[term_elab magma_expr] unsafe def elabMagmaExpr : TermElab := fun stx _ =>
+  match stx with
+  | `([magma| $vars:ident* | $tm:magma |]) => do
+    let u ← mkFreshLevelMVar
+    let tp ← mkFreshExprMVar none
+    mkMagmaExpr u tp vars tm
+  | _ => throwUnsupportedSyntax
+
+
+
+/-!
+# Common Terms
+-/
+
+-- a ρ ~~~~> .op (.op a ρ₀)
+
+def test (a : α) : FreeMagma α 3 := [magma| x y z | (x a) (x z) |]
+
+#print test
